sketch proof except for loop and ifthenelse

Pullback/SSA/Basic.lean
@@ -111,6 +111,8 @@ Fin.last' - Fin.cast (size_reverse) res) (as.reverse.findFinIdx? p)
 def Map.get {α β} [DecidableEq α] (map : Map α β) (key : α) : Option β :=
     map.findLast? (·.1 = key) |>.map (·.2)
 
+def Map.uniqueKeys {α β} [DecidableEq α] (x : Map α β) := (x.toList.map (·.1)).Nodup
+
 def SSABaseConst.inferType : SSABaseConst → SSABaseType
 | .float _ => .float
 | .int _ => .int
