Pullback/SSA/SSA.lean
@@ -28,19 +28,130 @@ theorem Array.mem_isPrefixOf {α} [BEq α] [LawfulBEq α] (as bs : Array α) : a
     have : x ∈ as.toList := hx.val
     grind only [= List.subset_def, = mem_toList_iff, #d8ea]
 
+#check Subtype.mk
+def Option.subtypeMap {α : Type} {P Q : α → Prop} (hP : ∀ x, P x → Q x) : Option (Subtype P) → Option (Subtype Q) :=
+    Option.map (Subtype.map _ hP)
+
+
+theorem Map.submap_get_uniqueKeys {α β} [DecidableEq α] (vars₁ vars₂ : Map α β) (hvars₁ : vars₁.uniqueKeys) :
+        vars₁.submap vars₂ → ∀ x ∈ vars₁, vars₂.get x.1 = some x.2 := by
+    intro hvars
+    simp only [submap, Array.any_eq_true', decide_eq_true_eq, Set.setOf_subset_setOf,
+     forall_exists_index] at hvars
+    have := hvars.2
+    intro x hx
+    specialize this x.1 x ⟨hx, (by grind)⟩
+    rw [← this]
+    exact get_uniqueKeys vars₁ hvars₁ x hx
+
+-- todo :: add hyps for alignment between the continutations in name and function form (kbreak and nkbreak)
+def SSADo.evalRefined {args mutArgs kmutArgs : ArgMap} {kbreak kcontinue : Option (ArgMap → Option SSAConst)} {vars mutVars kmutVars : VarMap} {nkbreak nkcontinue : Option Name}
+    (hMut : mutVars.uniqueKeys)
+    (hcontMutVars : kmutVars.isPrefixOf mutVars)
+    (halign : args.submapVars vars)
+    (halignMut : mutArgs.equivVars mutVars)
+    (halignkMut : kmutArgs.equivVars kmutVars) :
+    (prog : SSADo) →
+        Option {x : SSAConst //
+            (hkBreak : kbreak.All kmutArgs.validContinutation) →
+            (hkContinue : kcontinue.All kmutArgs.validContinutation) →
+            (hnkBreak : nkbreak.All (prog.validContinutationRef vars mutVars kmutVars)) →
+            (hnkContinue : nkcontinue.All (prog.validContinutationRef vars mutVars kmutVars)) →
+            x = (prog.toSSAExpr! vars mutVars kmutVars nkbreak nkcontinue).eval args}
+| expr e => do
+    match kcontinue with
+    | some kcontinue =>
+        -- todo :: don't discard `e` and use bind
+        (kcontinue kmutArgs).attachWith _
+            fun x hx => sorry
+    | none =>
+        (e.eval args).attachWith _
+            fun x hx => sorry
+| seq s₁ s₂ => do
+    let ⟨x, hx⟩ ← (s₁.eval args mutArgs kmutArgs kbreak kcontinue).attach
+    s₂.evalRefined hMut hcontMutVars halign halignMut halignkMut |>.subtypeMap
+        fun x hx => sorry
+| letE var val rest => do
+    if hvar : mutArgs.any (·.1 == var) then
+        -- cannot shadow mutVars
+        none
+    else
+        let ⟨valConst, hvalConst⟩ ← (val.eval args).attach
+        have halign' : ArgMap.submapVars (args.push (var, valConst)) (vars.push (var, val.inferType! vars)) := sorry
+        rest.evalRefined hMut hcontMutVars halign' halignMut halignkMut |>.subtypeMap
+            fun x hx => sorry
+| letM var val rest => do
+    if hvar : mutArgs.any (·.1 == var) then
+        -- cannot shadow mutVars
+        none
+    else
+        let ⟨val', hval'⟩ ← (val.eval args).attach
+        have halign' : ArgMap.submapVars (args.push (var, val')) (vars.push (var, val.inferType! vars)) := sorry
+        have halignMut' : ArgMap.equivVars (mutArgs.push (var, val')) (mutVars.push (var, val.inferType! vars)) := sorry
+        have hMut' : Map.uniqueKeys (mutVars.push (var, val.inferType! vars)) := sorry
+        have hcontMutVars' : Array.isPrefixOf kmutVars (Array.push mutVars (var, SSAExpr.inferType! vars val)) := sorry
+        rest.evalRefined hMut' hcontMutVars' halign' halignMut' halignkMut |>.subtypeMap
+            fun x hx => sorry
+| assign var val rest => do
+    let ⟨idx, hidx⟩ ← ((mutArgs).findFinIdx? (·.1 == var)).attach
+    let ⟨val', hval'⟩ ← (val.eval args).attach
+    if h : val'.inferType == mutArgs[idx].2.inferType then
+        -- we're changing value not the underlying type so alignment is perserved
+        have halignMut' : ArgMap.equivVars (mutArgs.set idx (var, val')) mutVars := by
+            sorry
+        rest.evalRefined hMut hcontMutVars halign halignMut' halignkMut |>.subtypeMap
+            fun x hx => sorry
+    else
+        none
+| loop body rest => do
+    let kMutArgs' := mutArgs
+    let ⟨kcontinue, hkcontinue⟩ ← kcontinue.attach
+    let kcontinue' :=
+        fun mutArgs' : Array (Name × SSAConst) =>
+            kcontinue (kMutArgs'.map (fun (n, _) => (n, (mutArgs'.findLast? (·.1 == n)).get!.2)))
+    SSA.loop mutArgs (fun mutArgs' kcont =>
+        body.eval (args ++ mutArgs') mutArgs' kMutArgs' kcontinue' kcont) |>.attachWith _
+            fun x hx => sorry
+| .break =>
+    match kbreak with
+    | some kbreak' => kbreak' mutArgs |>.attachWith _
+        fun x hx => sorry
+    | none => none
+| .continue =>
+    match kcontinue with
+    | some kcontinue' => kcontinue' mutArgs |>.attachWith _
+        fun x hx => sorry
+    | none => none
+| .return out =>
+    out.eval args |>.attachWith _
+        fun x hx => sorry
+| ifthenelse c t e rest => do
+    let kMutArgs' := mutArgs
+    let kcontinue' :=
+        fun mutArgs' : Array (Name × SSAConst) =>
+            let mutArgsNew : Array (Name × SSAConst) := (kMutArgs'.map (fun (n, _) => (n, (mutArgs'.findLast? (·.1 == n)).get!.2)))
+            rest.eval (args ++ mutArgsNew) mutArgsNew mutArgsNew kbreak kcontinue
+    match ← c.eval args with
+    | .ofBase (.int ci) =>
+        if ci != 0 then
+            t.eval args mutArgs kMutArgs' kbreak kcontinue'
+        else
+            e.eval args mutArgs kMutArgs kbreak kcontinue'
+    | _ => none
+
 theorem SSADo.eval_eq_eval_toSSAExpr! {kbreak kcontinue : Option (ArgMap → Option SSAConst)} {nkbreak nkcontinue : Option Name} {args mutArgs kmutArgs : ArgMap} {vars mutVars kmutVars : VarMap}
- (hMut₁ : (mutVars.toList.map (·.1)).Nodup) (hMut₂ : ∀ x ∈ mutVars, vars.get x.1 = some x.2)
- (hcontMutVars : kmutVars.isPrefixOf mutVars)
- (halign : args.submapVars vars)
- (halignMut : mutArgs.equivVars mutVars)
- (halignkMut : kmutArgs.equivVars kmutVars)
- (prog : SSADo)
- (hkBreak : kbreak.All kmutArgs.validContinutation)
- (hkContinue : kcontinue.All kmutArgs.validContinutation)
- (hnkBreak : nkbreak.All (prog.validContinutationRef vars mutVars kmutVars))
- (hnkContinue : nkcontinue.All (prog.validContinutationRef vars mutVars kmutVars)) :
-    ∀ x, prog.eval args mutArgs kmutArgs kbreak kcontinue = some x →
-        x = (prog.toSSAExpr! vars mutVars kmutVars nkbreak nkcontinue).eval args := sorry
+    (hMut₁ : (mutVars.toList.map (·.1)).Nodup) (hMut₂ : ∀ x ∈ mutVars, vars.get x.1 = some x.2)
+    (hcontMutVars : kmutVars.isPrefixOf mutVars)
+    (halign : args.submapVars vars)
+    (halignMut : mutArgs.equivVars mutVars)
+    (halignkMut : kmutArgs.equivVars kmutVars) :
+    (prog : SSADo) →
+    (hkBreak : kbreak.All kmutArgs.validContinutation) →
+    (hkContinue : kcontinue.All kmutArgs.validContinutation) →
+    (hnkBreak : nkbreak.All (prog.validContinutationRef vars mutVars kmutVars)) →
+    (hnkContinue : nkcontinue.All (prog.validContinutationRef vars mutVars kmutVars)) →
+        ∀ x, prog.eval args mutArgs kmutArgs kbreak kcontinue = some x →
+            x = (prog.toSSAExpr! vars mutVars kmutVars nkbreak nkcontinue).eval args := by sorry
 /-
      IR.eval
    IR ----> Const
